assembly/OpCodes2.v
@@ -1,0 +1,46 @@
+Require Import Utf8.
+
+Require Import Assembly.Bits.
+Require Assembly.OpCodes.
+
+Notation EXIT := (toB8 OpCodes.EXIT).
+Notation NOP := (toB8 OpCodes.NOP).
+Notation JUMP := (toB8 OpCodes.JUMP).
+Notation JUMP_ZERO := (toB8 OpCodes.JUMP_ZERO).
+Notation SET_SP := (toB8 OpCodes.SET_SP).
+Notation GET_PC := (toB8 OpCodes.GET_PC).
+Notation GET_SP := (toB8 OpCodes.GET_SP).
+Notation PUSH0 := (toB8 OpCodes.PUSH0).
+Notation PUSH1 := (toB8 OpCodes.PUSH1).
+Notation PUSH2 := (toB8 OpCodes.PUSH2).
+Notation PUSH4 := (toB8 OpCodes.PUSH4).
+Notation PUSH8 := (toB8 OpCodes.PUSH8).
+Notation SIGX1 := (toB8 OpCodes.SIGX1).
+Notation SIGX2 := (toB8 OpCodes.SIGX2).
+Notation SIGX4 := (toB8 OpCodes.SIGX4).
+Notation LOAD1 := (toB8 OpCodes.LOAD1).
+Notation LOAD2 := (toB8 OpCodes.LOAD2).
+Notation LOAD4 := (toB8 OpCodes.LOAD4).
+Notation LOAD8 := (toB8 OpCodes.LOAD8).
+Notation STORE1 := (toB8 OpCodes.STORE1).
+Notation STORE2 := (toB8 OpCodes.STORE2).
+Notation STORE4 := (toB8 OpCodes.STORE4).
+Notation STORE8 := (toB8 OpCodes.STORE8).
+Notation ADD := (toB8 OpCodes.ADD).
+Notation MULT := (toB8 OpCodes.MULT).
+Notation DIV := (toB8 OpCodes.DIV).
+Notation REM := (toB8 OpCodes.REM).
+Notation LT := (toB8 OpCodes.LT).
+Notation AND := (toB8 OpCodes.AND).
+Notation OR := (toB8 OpCodes.OR).
+Notation NOT := (toB8 OpCodes.NOT).
+Notation XOR := (toB8 OpCodes.XOR).
+Notation POW2 := (toB8 OpCodes.POW2).
+
+Notation READ_FRAME := (toB8 OpCodes.READ_FRAME).
+Notation READ_PIXEL := (toB8 OpCodes.READ_PIXEL).
+Notation NEW_FRAME := (toB8 OpCodes.NEW_FRAME).
+Notation SET_PIXEL := (toB8 OpCodes.SET_PIXEL).
+Notation ADD_SAMPLE := (toB8 OpCodes.ADD_SAMPLE).
+Notation PUT_CHAR := (toB8 OpCodes.PUT_CHAR).
+Notation PUT_BYTE := (toB8 OpCodes.PUT_BYTE).
